SizeLemmas.v
@@ -8,6 +8,8 @@ Require Import Omega.
 (* see file ReducibilityMeasure for the full measure *)
 Fixpoint typeNodes T: nat :=
   match T with
+  | ite b T1 T2 => 1 + typeNodes T1 + typeNodes T2
+
   | T_unit => 0
   | T_bool => 0
   | T_nat => 0
@@ -27,18 +29,24 @@ Fixpoint typeNodes T: nat :=
   | T_exists A B => 1 + typeNodes A + typeNodes B
   | T_abs T => 1 + typeNodes T
   | T_rec _ T0 Ts => 1 + typeNodes T0 + typeNodes Ts
+  | T_interpret T => 1 + typeNodes T
 
   | _ => 0
   end.
 
+(*
 Lemma typeNodes_term_form:
   forall t, is_erased_term t -> typeNodes t = 0.
 Proof.
   destruct t; steps.
 Qed.
+*)
 
 Lemma typeNodes_opening:
-  forall T k rep, is_erased_term rep -> typeNodes (open k T rep) = typeNodes T.
+  forall T k rep,
+    is_erased_type T ->
+    is_erased_term rep ->
+    typeNodes (open k T rep) = typeNodes T.
 Proof.
   induction T; repeat step || rewrite_any || apply typeNodes_term_form;
     try omega.
@@ -69,3 +77,66 @@ Proof.
 Qed.
 
 Hint Rewrite typeNodes_swap: bsize.
+
+Fixpoint count_interpret (t: tree): nat :=
+  match t with
+  | ite b T1 T2 => count_interpret T1 + count_interpret T2
+
+  | T_refine A p => count_interpret A
+  | T_type_refine A B => count_interpret A + count_interpret B
+  | T_prod A B => count_interpret A + count_interpret B
+  | T_arrow A B => count_interpret A + count_interpret B
+  | T_sum A B => count_interpret A + count_interpret B
+  | T_let t B => count_interpret B
+  | T_intersection A B => count_interpret A + count_interpret B
+  | T_union A B => count_interpret A + count_interpret B
+  | T_forall A B => count_interpret A + count_interpret B
+  | T_exists A B => count_interpret A + count_interpret B
+  | T_abs T => count_interpret T
+  | T_rec n T0 Ts => count_interpret T0 + count_interpret Ts
+  | T_interpret t => 1 + count_interpret t
+  | _ => 0
+  end.
+
+(*
+Lemma count_interpret_term:
+  forall t, is_erased_term t -> count_interpret t = 0.
+Proof.
+  destruct t; steps.
+Qed.
+*)
+
+Lemma count_interpret_open:
+  forall T k rep,
+    is_erased_type T ->
+    is_erased_term rep ->
+    count_interpret (open k T rep) = count_interpret T.
+Proof.
+  induction T; repeat step || rewrite_any; try omega.
+Qed.
+
+Hint Rewrite count_interpret_open: bsize.
+
+Lemma count_interpret_open_var:
+  forall T k X, count_interpret (open k T (fvar X type_var)) = count_interpret T.
+Proof.
+  induction T; steps.
+Qed.
+
+Hint Rewrite count_interpret_open_var: bsize.
+
+Lemma count_interpret_topen_var:
+  forall T k X, count_interpret (topen k T (fvar X type_var)) = count_interpret T.
+Proof.
+  induction T; steps.
+Qed.
+
+Hint Rewrite count_interpret_topen_var: bsize.
+
+Lemma count_interpret_swap:
+  forall t i j, count_interpret (swap_type_holes t i j) = count_interpret t.
+Proof.
+  induction t; steps.
+Qed.
+
+Hint Rewrite count_interpret_swap: bsize.
